sample-emit5.bpl
@@ -1,0 +1,882 @@
+type $Bool = bool;
+type $Int32 = bv32;
+type $Double = float53e11; // 64-bit; see https://github.com/boogie-org/boogie/issues/29#issuecomment-231239065
+
+function {:bvbuiltin "bvadd"} $Int32^Add(x: $Int32, y: $Int32): $Int32;
+// etc; see https://boogie-docs.readthedocs.io/en/latest/LangRef.html#other-operators
+
+type {:datatype} $ValueType;
+function {:constructor} $ValueType~Double(): $ValueType;
+function {:constructor} $ValueType~Int32(): $ValueType;
+function {:constructor} $ValueType~Boolean(): $ValueType;
+function {:constructor} $ValueType~Undefined(): $ValueType;
+function {:constructor} $ValueType~Null(): $ValueType;
+function {:constructor} $ValueType~Magic(): $ValueType;
+function {:constructor} $ValueType~String(): $ValueType;
+function {:constructor} $ValueType~Symbol(): $ValueType;
+function {:constructor} $ValueType~PrivateGCThing(): $ValueType;
+function {:constructor} $ValueType~BigInt(): $ValueType;
+function {:constructor} $ValueType~Object(): $ValueType;
+
+type $Value;
+
+function $Value~typeOf($value: $Value): $ValueType;
+
+procedure $Value~isDouble($value: $Value)
+  returns (ret: $Bool)
+{
+  ret := $Value~typeOf($value) == $ValueType~Double();
+}
+
+procedure $Value~fromDouble($double: $Double)
+  returns (ret: $Value)
+{
+  var $value: $Value;
+  var tmp'0: $Bool;
+  $value := $Value~fromDoubleUnchecked($double);
+  call tmp'0 := $Value~isDouble($value);
+  assume tmp'0;
+  assume $Value~toDoubleUnchecked($value) == $double;
+  ret := $value;
+}
+
+function $Value~fromDoubleUnchecked($double: $Double): $Value;
+
+procedure $Value~toDouble($value: $Value)
+  returns (ret: $Double)
+{
+  var $double: $Double;
+  var tmp'0: $Bool;
+  call tmp'0 := $Value~isDouble($value);
+  assert tmp'0;
+  $double := $Value~toDoubleUnchecked($value);
+  assume $Value~fromDoubleUnchecked($double) == $value;
+  ret := $double;
+}
+
+function $Value~toDoubleUnchecked($value: $Value): $Double;
+
+procedure $Value~isInt32($value: $Value)
+  returns (ret: $Bool)
+{
+  ret := $Value~typeOf($value) == $ValueType~Int32();
+}
+
+procedure $Value~fromInt32($int32: $Int32)
+  returns (ret: $Value)
+{
+  var $value: $Value;
+  var tmp'0: $Bool;
+  $value := $Value~fromInt32Unchecked($int32);
+  call tmp'0 := $Value~isInt32($value);
+  assume tmp'0;
+  assume $Value~toInt32Unchecked($value) == $int32;
+  ret := $value;
+}
+
+function $Value~fromInt32Unchecked($int32: $Int32): $Value;
+
+procedure $Value~toInt32($value: $Value)
+  returns (ret: $Int32)
+{
+  var $int32: $Int32;
+  var tmp'0: $Bool;
+  call tmp'0 := $Value~isInt32($value);
+  assert tmp'0;
+  $int32 := $Value~toInt32Unchecked($value);
+  assume $Value~fromInt32Unchecked($int32) == $value;
+  ret := $int32;
+}
+
+function $Value~toInt32Unchecked($value: $Value): $Int32;
+
+procedure $Value~isBoolean($value: $Value)
+  returns (ret: $Bool)
+{
+  ret := $Value~typeOf($value) == $ValueType~Boolean();
+}
+
+procedure $Value~fromBoolean($boolean: $Bool)
+  returns (ret: $Value)
+{
+  var $value: $Value;
+  var tmp'0: $Bool;
+  $value := $Value~fromBooleanUnchecked($boolean);
+  call tmp'0 := $Value~isBoolean($value);
+  assume tmp'0;
+  assume $Value~toBooleanUnchecked($value) == $boolean;
+  ret := $value;
+}
+
+function $Value~fromBooleanUnchecked($boolean: $Bool): $Value;
+
+procedure $Value~toBoolean($value: $Value)
+  returns (ret: $Bool)
+{
+  var $boolean: $Bool;
+  var tmp'0: $Bool;
+  call tmp'0 := $Value~isBoolean($value);
+  assert tmp'0;
+  $boolean := $Value~toBooleanUnchecked($value);
+  assume $Value~fromBooleanUnchecked($boolean) == $value;
+  ret := $boolean;
+}
+
+function $Value~toBooleanUnchecked($value: $Value): $Bool;
+
+procedure $Value~isNull($value: $Value)
+  returns (ret: $Bool)
+{
+  ret := $Value~typeOf($value) == $ValueType~Null();
+}
+
+procedure $Value~isMagic($value: $Value)
+  returns (ret: $Bool)
+{
+  ret := $Value~typeOf($value) == $ValueType~Magic();
+}
+
+procedure $Value~isObject($value: $Value)
+  returns (ret: $Bool)
+{
+  ret := $Value~typeOf($value) == $ValueType~Object();
+}
+
+procedure $Value~fromObject($object: $Object)
+  returns (ret: $Value)
+{
+  var $value: $Value;
+  var tmp'0: $Bool;
+  $value := $Value~fromObjectUnchecked($object);
+  call tmp'0 := $Value~isObject($value);
+  assume tmp'0;
+  assume $Value~toObjectUnchecked($value) == $object;
+  ret := $value;
+}
+
+function $Value~fromObjectUnchecked($object: $Object): $Value;
+
+procedure $Value~toObject($value: $Value)
+  returns (ret: $Object)
+{
+  var $object: $Object;
+  var tmp'0: $Bool;
+  call tmp'0 := $Value~isObject($value);
+  assert tmp'0;
+  $object := $Value~toObjectUnchecked($value);
+  assume $Value~fromObjectUnchecked($object) == $value;
+  ret := $object;
+}
+
+function $Value~toObjectUnchecked($value: $Value): $Object;
+
+type $Object;
+
+function $Object~shapeOf($object: $Object): $Shape;
+
+procedure $Object~getProto($object: $Object)
+  returns (ret: $Value)
+{
+  var $proto: $Value;
+  var tmp'0: $Bool;
+  var tmp'1: $Bool;
+  var tmp'2: $Bool;
+  $proto := $Object~getProtoUnchecked($object);
+  call tmp'0 := $Value~isObject($proto);
+  call tmp'1 := $Value~isNull($proto);
+  call tmp'2 := $Value~isMagic($proto);
+  assume tmp'0 || tmp'1 || tmp'2;
+  ret := $proto;
+  return;
+}
+
+function $Object~getProtoUnchecked($object: $Object): $Value;
+
+procedure $Object~toNativeObject($object: $Object)
+  returns (ret: $NativeObject)
+{
+  var $shape: $Shape;
+  var $class: $Class;
+  $shape := $Object~shapeOf($object);
+  $class := $Shape~classOf($shape);
+  assert $Class~isNativeObject($class);
+  ret := $NativeObject^from$Object($object);
+}
+
+procedure $Object~getFixedSlot($object: $Object, $slot: $Int32)
+  returns (ret: $Value)
+{
+  var $nativeObject: $NativeObject;
+  var tmp'0: $NativeObject;
+  var tmp'1: $Value;
+  call tmp'0 := $Object~toNativeObject($object);
+  $nativeObject := tmp'0;
+  call tmp'1 := $NativeObject~getFixedSlot($nativeObject, $slot);
+  ret := tmp'1;
+}
+
+type $NativeObject;
+
+function $NativeObject^from$Object(in: $Object): $NativeObject;
+function $NativeObject^to$Object(in: $NativeObject): $Object;
+axiom (forall in: $NativeObject :: $NativeObject^from$Object($NativeObject^to$Object(in)) == in);
+axiom (forall in: $Object :: $NativeObject^to$Object($NativeObject^from$Object(in)) == in);
+
+procedure $NativeObject~getFixedSlot($nativeObject: $NativeObject, $slot: $Int32)
+  returns (ret: $Value)
+{
+  var $shape: $Shape;
+  $shape := $Object~shapeOf($NativeObject^to$Object($nativeObject));
+  assert $Shape~hasFixedSlot($shape, $slot);
+  ret := $NativeObject~getFixedSlotUnchecked($nativeObject, $slot);
+}
+
+function $NativeObject~getFixedSlotUnchecked($nativeObject: $NativeObject, $slot: $Int32): $Value;
+
+type $Shape;
+
+function $Shape~classOf($shape: $Shape): $Class;
+
+function $Shape~hasFixedSlot($shape: $Shape, $slot: $Int32): $Bool;
+
+type $Class;
+
+function $Class~isNativeObject($class: $Class): $Bool;
+
+type $ValueReg;
+type ValueRegs = [$ValueReg]$Value;
+
+procedure $ValueReg~getValue(valueRegs: ValueRegs, $valueReg: $ValueReg)
+  returns (ret: $Value)
+{ 
+  ret := valueRegs[$valueReg];
+}
+
+procedure $ValueReg~setValue(valueRegs: ValueRegs, $valueReg: $ValueReg, $value: $Value)
+  returns (out_valueRegs: ValueRegs)
+{
+  out_valueRegs := valueRegs;
+  out_valueRegs[$valueReg] := $value;
+}
+
+type $Reg;
+type Regs = [$Reg]$Value;
+
+procedure $Reg~getBoolean(regs: Regs, $reg: $Reg)
+  returns (ret: $Bool)
+{ 
+  var tmp'0: $Bool;
+  call tmp'0 := $Value~toBoolean(regs[$reg]);
+  ret := tmp'0;
+}
+
+procedure $Reg~setBoolean(regs: Regs, $reg: $Reg, $boolean: $Bool)
+  returns (out_regs: Regs)
+{
+  var tmp'0: $Value;
+  call tmp'0 := $Value~fromBoolean($boolean);
+  out_regs := regs;
+  out_regs[$reg] := tmp'0;
+}
+
+procedure $Reg~getObject(regs: Regs, $reg: $Reg)
+  returns (ret: $Object)
+{ 
+  var tmp'0: $Object;
+  call tmp'0 := $Value~toObject(regs[$reg]);
+  ret := tmp'0;
+}
+
+procedure $Reg~setObject(regs: Regs, $reg: $Reg, $object: $Object)
+  returns (out_regs: Regs)
+{
+  var tmp'0: $Value;
+  call tmp'0 := $Value~fromObject($object);
+  out_regs := regs;
+  out_regs[$reg] := tmp'0;
+}
+
+type {:datatype} $MASM^Op;
+//function {:constructor} $MASM^Op^noOp(): $MASM^Op;
+
+type $MASM^Pc = int;
+
+var $MASM^pc: $MASM^Pc;
+
+procedure {:inline 1} $MASM^step()
+  modifies $MASM^pc;
+{
+  $MASM^pc := $MASM^pc + 1;
+}
+
+type $MASM^Label = int;
+
+var $MASM^nextLabel: $MASM^Label;
+var $MASM^labels: [$MASM^Label]$MASM^Pc;
+
+procedure $MASM^label()
+  returns (label: $MASM^Label)
+  modifies $MASM^nextLabel;
+{
+  label := $MASM^nextLabel;
+  $MASM^nextLabel := $MASM^nextLabel + 1;
+}
+
+type $MASM^Bind = int;
+
+var $MASM^pcBinds: [$MASM^Pc]$MASM^Bind;
+
+procedure {:inline 1} $MASM^bind(bind: $MASM^Bind, label: $MASM^Label)
+  modifies $MASM^labels;
+{
+  $MASM^pcBinds[$MASM^emitPc] := bind;
+  $MASM^labels[label] := $MASM^emitPc;
+}
+
+procedure {:inline 1} $MASM^jump(label: $MASM^Label)
+  modifies $MASM^pc;
+{
+  $MASM^pc := $MASM^labels[label];
+}
+
+var $MASM^emitPc: $MASM^Pc;
+var $MASM^emitOps: [$MASM^Pc]$MASM^Op;
+var $MASM^emitTrace: [$MASM^Pc]bool;
+
+procedure $MASM^emit(op: $MASM^Op)
+  modifies $MASM^emitOps;
+  modifies $MASM^emitPc;
+{
+  $MASM^emitOps[$MASM^emitPc] := op;
+  $MASM^emitPc := $MASM^emitPc + 1;
+}
+
+procedure $MASM^record(branch: bool)
+  modifies $MASM^emitTrace;
+{
+  $MASM^emitTrace[$MASM^emitPc] := branch;
+}
+
+function {:constructor} $MASM^Op~jump($label: $MASM^Label): $MASM^Op;
+
+function {:constructor} $MASM^Op~storeBoolean($boolean: $Bool, $dstReg: $Reg): $MASM^Op;
+
+procedure $MASM~storeBoolean(regs: Regs, $boolean: $Bool, $dstReg: $Reg)
+  returns (out_regs: Regs)
+  //modifies $MASM^pc;
+{
+  call out_regs := $Reg~setBoolean(regs, $dstReg, $boolean);
+  call $MASM^step();
+}
+
+function {:constructor} $MASM^Op~branchTestNull($valueReg: $ValueReg, $label: $MASM^Label): $MASM^Op;
+
+function {:constructor} $MASM^Op~branchTestMagic($valueReg: $ValueReg, $label: $MASM^Label): $MASM^Op;
+
+function {:constructor} $MASM^Op~branchTestNotObject($valueReg: $ValueReg, $label: $MASM^Label): $MASM^Op;
+
+function {:constructor} $MASM^Op~unboxObject($valueReg: $ValueReg, $objectReg: $Reg): $MASM^Op;
+
+procedure $MASM~unboxObject(valueRegs: ValueRegs, regs: Regs, $valueReg: $ValueReg, $objectReg: $Reg)
+  returns (out_regs: Regs)
+  modifies $MASM^pc;
+{
+  var $value: $Value;
+  var tmp'0: $Value;
+  var tmp'1: $Object;
+  call tmp'0 := $ValueReg~getValue(valueRegs, $valueReg);
+  $value := tmp'0;
+  call tmp'1 := $Value~toObject($value);
+  call out_regs := $Reg~setObject(regs, $objectReg, tmp'1);
+  call $MASM^step();
+}
+
+function {:constructor} $MASM^Op~branchTestObjectEq($lhsReg: $Reg, $rhsReg: $Reg, $label: $MASM^Label): $MASM^Op;
+
+function {:constructor} $MASM^Op~loadObjectProto($objectReg: $Reg, $protoReg: $ValueReg): $MASM^Op;
+
+procedure $MASM~loadObjectProto(valueRegs: ValueRegs, regs: Regs, $objectReg: $Reg, $protoReg: $ValueReg)
+  returns (out_valueRegs: ValueRegs)
+  //modifies $MASM^pc;
+{
+  var $object: $Object;
+  var tmp'0: $Object;
+  var tmp'1: $Value;
+  call tmp'0 := $Reg~getObject(regs, $objectReg);
+  $object := tmp'0;
+  call tmp'1 := $Object~getProto($object);
+  call out_valueRegs := $ValueReg~setValue(valueRegs, $protoReg, tmp'1);
+  call $MASM^step();
+}
+
+type $ValId;
+
+function $ValId~toValueReg($valId: $ValId): $ValueReg;
+
+type $ObjId;
+
+function $ObjId~toReg($objId: $ObjId): $Reg;
+
+type $Int32Field;
+
+function $Int32Field~toInt32($int32Field: $Int32Field): $Int32;
+
+type $ShapeField;
+
+function $ShapeField~toShape($shapeField: $ShapeField): $Shape;
+
+procedure $CacheIR~loadInstanceOfObjectResult($lhsId: $ValId, $protoId: $ObjId, $scratch: $Reg, $output: $Reg, $failure: $MASM^Label)
+  modifies $MASM^emitPc;
+  modifies $MASM^emitOps;
+{
+  var $lhs: $ValueReg;
+  var $proto: $Reg;
+  var $loop: $MASM^Label;
+  var $returnFalse: $MASM^Label;
+  var $returnTrue: $MASM^Label;
+  var $done: $MASM^Label;
+
+  $lhs := $ValId~toValueReg($lhsId);
+  $proto := $ObjId~toReg($protoId);
+
+  call $loop := $MASM^label();
+  call $returnFalse := $MASM^label();
+  call $returnTrue := $MASM^label();
+  call $done := $MASM^label();
+
+  call $MASM^emit($MASM^Op~branchTestNotObject($lhs, $returnFalse));
+  call $MASM^emit($MASM^Op~unboxObject($lhs, $scratch));
+  call $MASM^emit($MASM^Op~loadObjectProto($scratch, $lhs));
+
+  call $MASM^bind(1, $loop);
+  call $MASM^emit($MASM^Op~branchTestNull($lhs, $returnFalse));
+  call $MASM^emit($MASM^Op~branchTestMagic($lhs, $failure));
+
+  call $MASM^emit($MASM^Op~branchTestNotObject($lhs, $returnFalse));
+  call $MASM^emit($MASM^Op~unboxObject($lhs, $scratch));
+  call $MASM^emit($MASM^Op~branchTestObjectEq($scratch, $proto, $returnTrue));
+
+  call $MASM^emit($MASM^Op~loadObjectProto($scratch, $lhs));
+  call $MASM^emit($MASM^Op~jump($loop));
+
+  call $MASM^bind(2, $returnFalse);
+  call $MASM^emit($MASM^Op~storeBoolean(false, $output));
+  call $MASM^emit($MASM^Op~jump($done));
+
+  call $MASM^bind(3, $returnTrue);
+  call $MASM^emit($MASM^Op~storeBoolean(true, $output));
+
+  call $MASM^bind(4, $done);
+}
+
+const $shape: $Shape;
+const $class: $Class;
+const $slot: $Int32;
+
+axiom $Shape~hasFixedSlot($shape, $slot);
+axiom $Shape~classOf($shape) == $class;
+axiom $Class~isNativeObject($class);
+
+const $shapeField: $ShapeField;
+const $slotField: $Int32Field;
+
+axiom $ShapeField~toShape($shapeField) == $shape;
+axiom $Int32Field~toInt32($slotField) == $slot;
+
+procedure {:entrypoint} $InstanceOf2($lhsId: $ValId, $protoId: $ObjId, $scratch: $Reg, $output: $Reg)
+  modifies $MASM^emitPc;
+  modifies $MASM^emitOps;
+{
+  var op: $MASM^Op;
+
+  var valueRegs: ValueRegs;
+  var regs: Regs;
+
+  var $failure: $MASM^Label;
+
+  var $lhs: $ValueReg;
+  var lhs: $Value;
+  var $proto: $Reg;
+  var proto: $Object;
+  var scratch: $Object;
+  var b: $Bool;
+
+  var $MASM~branchTestNull'$value: $Value;
+  var $MASM~branchTestNull'tmp'0: $Value;
+  var $MASM~branchTestNull'tmp'1: $Bool;
+
+  var $MASM~branchTestMagic'$value: $Value;
+  var $MASM~branchTestMagic'tmp'0: $Value;
+  var $MASM~branchTestMagic'tmp'1: $Bool;
+
+  var $MASM~branchTestNotObject'$value: $Value;
+  var $MASM~branchTestNotObject'tmp'0: $Value;
+  var $MASM~branchTestNotObject'tmp'1: $Bool;
+
+  var $MASM~branchTestObjectEq'$lhs: $Object;
+  var $MASM~branchTestObjectEq'$rhs: $Object;
+  var $MASM~branchTestObjectEq'tmp'0: $Object;
+  var $MASM~branchTestObjectEq'tmp'1: $Object;
+
+  $lhs := $ValId~toValueReg($lhsId);
+  $proto := $ObjId~toReg($protoId);
+
+  assume $proto != $scratch;
+  assume $Value~typeOf(regs[$proto]) == $ValueType~Object();
+
+  call proto := $Reg~getObject(regs, $proto);
+
+  $MASM^emitPc := 0;
+
+  assume (forall pc: $MASM^Pc :: $MASM^pcBinds[pc] == -1);
+
+  call $failure := $MASM^label();
+
+  call $CacheIR~loadInstanceOfObjectResult($lhsId, $protoId, $scratch, $output, $failure);
+
+  $MASM^emitPc := $MASM^emitPc + 1;
+
+  call $MASM^bind(0, $failure);
+  $MASM^emitPc := $MASM^emitPc + 1;
+
+  assert $MASM^emitPc >= 0;
+
+  $MASM^pc := 0;
+
+  op'0$MASM~branchTestNotObject:
+    op := $MASM^emitOps[$MASM^pc];
+    call $MASM~branchTestNotObject'tmp'0 := $ValueReg~getValue(valueRegs, $valueReg#$MASM^Op~branchTestNotObject(op));
+    $MASM~branchTestNotObject'$value := $MASM~branchTestNotObject'tmp'0;
+    call $MASM~branchTestNotObject'tmp'1 := $Value~isObject($MASM~branchTestNotObject'$value);
+    if (!$MASM~branchTestNotObject'tmp'1) {
+      call $MASM^jump($label#$MASM^Op~branchTestNotObject(op));
+      goto label$returnFalse;
+    }
+    call $MASM^step();
+
+  op'1$MASM~unboxObject:
+    op := $MASM^emitOps[$MASM^pc];
+    call regs := $MASM~unboxObject(
+      valueRegs,
+      regs,
+      $valueReg#$MASM^Op~unboxObject(op),
+      $objectReg#$MASM^Op~unboxObject(op)
+    );
+
+  op'2$MASM~loadObjectProto:
+    op := $MASM^emitOps[$MASM^pc];
+    call valueRegs := $MASM~loadObjectProto(
+      valueRegs,
+      regs,
+      $objectReg#$MASM^Op~loadObjectProto(op),
+      $protoReg#$MASM^Op~loadObjectProto(op)
+    );
+
+  assert regs[$proto] == $Value~fromObjectUnchecked(proto);
+
+  label$loop:
+    assume $MASM^pcBinds[$MASM^pc] == 1;
+    assume regs[$proto] == $Value~fromObjectUnchecked(proto);
+
+  op'3$MASM^branchTestNull:
+    op := $MASM^emitOps[$MASM^pc];
+    call $MASM~branchTestNull'tmp'0 := $ValueReg~getValue(valueRegs, $valueReg#$MASM^Op~branchTestNull(op));
+    $MASM~branchTestNull'$value := $MASM~branchTestNull'tmp'0;
+    call $MASM~branchTestNull'tmp'1 := $Value~isNull($MASM~branchTestNull'$value);
+    if ($MASM~branchTestNull'tmp'1) {
+      call $MASM^jump($label#$MASM^Op~branchTestNull(op));
+      goto label$returnFalse;
+    }
+    call $MASM^step();
+
+  op'4$MASM~branchTestMagic:
+    op := $MASM^emitOps[$MASM^pc];
+    call $MASM~branchTestMagic'tmp'0 := $ValueReg~getValue(valueRegs, $valueReg#$MASM^Op~branchTestMagic(op));
+    $MASM~branchTestMagic'$value := $MASM~branchTestMagic'tmp'0;
+    call $MASM~branchTestMagic'tmp'1 := $Value~isMagic($MASM~branchTestMagic'$value);
+    if ($MASM~branchTestMagic'tmp'1) {
+      call $MASM^jump($label#$MASM^Op~branchTestMagic(op));
+      goto label$failure;
+    }
+    call $MASM^step();
+
+  op'5$MASM~branchTestNotObject:
+    op := $MASM^emitOps[$MASM^pc];
+    call $MASM~branchTestNotObject'tmp'0 := $ValueReg~getValue(valueRegs, $valueReg#$MASM^Op~branchTestNotObject(op));
+    $MASM~branchTestNotObject'$value := $MASM~branchTestNotObject'tmp'0;
+    call $MASM~branchTestNotObject'tmp'1 := $Value~isObject($MASM~branchTestNotObject'$value);
+    if (!$MASM~branchTestNotObject'tmp'1) {
+      call $MASM^jump($label#$MASM^Op~branchTestNotObject(op));
+      goto label$returnFalse;
+    }
+    call $MASM^step();
+
+  op'6$MASM~unboxObject:
+    op := $MASM^emitOps[$MASM^pc];
+    call regs := $MASM~unboxObject(
+      valueRegs,
+      regs,
+      $valueReg#$MASM^Op~unboxObject(op),
+      $objectReg#$MASM^Op~unboxObject(op)
+    );
+
+  op'7$MASM~branchTestObjectEq:
+    op := $MASM^emitOps[$MASM^pc];
+    call $MASM~branchTestObjectEq'tmp'0 := $Reg~getObject(regs, $lhsReg#$MASM^Op~branchTestObjectEq(op));
+    $MASM~branchTestObjectEq'$lhs := $MASM~branchTestObjectEq'tmp'0;
+    call $MASM~branchTestObjectEq'tmp'1 := $Reg~getObject(regs, $rhsReg#$MASM^Op~branchTestObjectEq(op));
+    $MASM~branchTestObjectEq'$rhs := $MASM~branchTestObjectEq'tmp'1;
+    if ($MASM~branchTestObjectEq'$lhs == $MASM~branchTestObjectEq'$rhs) {
+      call $MASM^jump($label#$MASM^Op~branchTestObjectEq(op));
+      goto label$returnTrue;
+    }
+    call $MASM^step();
+
+  op'8$MASM~loadObjectProto:
+    op := $MASM^emitOps[$MASM^pc];
+    call valueRegs := $MASM~loadObjectProto(
+      valueRegs,
+      regs,
+      $objectReg#$MASM^Op~loadObjectProto(op),
+      $protoReg#$MASM^Op~loadObjectProto(op)
+    );
+
+  op'9$MASM~jump:
+    op := $MASM^emitOps[$MASM^pc];
+    call $MASM^jump($label#$MASM^Op~jump(op));
+    assert regs[$proto] == $Value~fromObjectUnchecked(proto);
+    goto label$loop;
+
+  label$returnFalse:
+    assume $MASM^pcBinds[$MASM^pc] == 2;
+
+  op'10$MASM~storeBoolean:
+    op := $MASM^emitOps[$MASM^pc];
+    call regs := $MASM~storeBoolean(
+      regs,
+      $boolean#$MASM^Op~storeBoolean(op),
+      $dstReg#$MASM^Op~storeBoolean(op)
+    );
+
+  op'11$MASM~jump:
+    op := $MASM^emitOps[$MASM^pc];
+    call $MASM^jump($label#$MASM^Op~jump(op));
+    goto label$done;
+
+  label$returnTrue:
+    assume $MASM^pcBinds[$MASM^pc] == 3;
+
+  op'12$MASM~storeBoolean:
+    op := $MASM^emitOps[$MASM^pc];
+    call regs := $MASM~storeBoolean(
+      regs,
+      $boolean#$MASM^Op~storeBoolean(op),
+      $dstReg#$MASM^Op~storeBoolean(op)
+    );
+
+  label$done:
+    assume $MASM^pcBinds[$MASM^pc] == 4;
+
+    return;
+
+  label$failure:
+    assume $MASM^pcBinds[$MASM^pc] == 0;
+}
+
+
+procedure /*{:entrypoint}*/ $InstanceOf($lhsId: $ValId, $protoId: $ObjId, $scratch: $Reg, $output: $Reg)
+  modifies $MASM^emitPc;
+  modifies $MASM^emitOps;
+  modifies $MASM^emitTrace;
+  //modifies $MASM^pc;
+{
+  var ops: [$MASM^Pc]$MASM^Op;
+  var op: $MASM^Op;
+
+  var valueRegs: ValueRegs;
+  var regs: Regs;
+
+  var $failure: $MASM^Label;
+
+  var $MASM~branchTestNull'$value: $Value;
+  var $MASM~branchTestNull'tmp'0: $Value;
+  var $MASM~branchTestNull'tmp'1: $Bool;
+
+  var $MASM~branchTestMagic'$value: $Value;
+  var $MASM~branchTestMagic'tmp'0: $Value;
+  var $MASM~branchTestMagic'tmp'1: $Bool;
+
+  var $MASM~branchTestNotObject'$value: $Value;
+  var $MASM~branchTestNotObject'tmp'0: $Value;
+  var $MASM~branchTestNotObject'tmp'1: $Bool;
+
+  var $MASM~branchTestObjectEq'$lhs: $Object;
+  var $MASM~branchTestObjectEq'$rhs: $Object;
+  var $MASM~branchTestObjectEq'tmp'0: $Object;
+  var $MASM~branchTestObjectEq'tmp'1: $Object;
+
+  /*
+  var origOutput: $Bool;
+  var origFailure: $Bool;
+  */
+
+  var initProtoId: $Bool;
+  call initProtoId := $Value~isObject(regs[$ObjId~toReg($protoId)]);
+  assume initProtoId;
+
+  assume $ObjId~toReg($protoId) != $scratch;
+
+  //call origOutput, origFailure := loadInstanceOfObjectResult($lhsId, $protoId);
+
+  //assume (forall pc: $MASM^Pc :: $MASM^emitOps[pc] == $MASM^Op^noOp());
+
+  $MASM^emitPc := 0;
+
+  call $failure := $MASM^label();
+
+  call $CacheIR~loadInstanceOfObjectResult($lhsId, $protoId, $scratch, $output, $failure);
+
+  $MASM^emitPc := $MASM^emitPc + 1;
+
+  call $MASM^bind(0, $failure);
+  $MASM^emitPc := $MASM^emitPc + 1;
+
+  assert $MASM^emitPc >= 0;
+
+  //$MASM^pc := 0;
+
+  ops := $MASM^emitOps;
+
+  op'0$MASM~branchTestNotObject:
+    op := ops[0];
+    call $MASM~branchTestNotObject'tmp'0 := $ValueReg~getValue(valueRegs, $valueReg#$MASM^Op~branchTestNotObject(op));
+    $MASM~branchTestNotObject'$value := $MASM~branchTestNotObject'tmp'0;
+    call $MASM~branchTestNotObject'tmp'1 := $Value~isObject($MASM~branchTestNotObject'$value);
+    if (!$MASM~branchTestNotObject'tmp'1) {
+      //call $MASM^jump($label#$MASM^Op~branchTestNotObject(op));
+      //$MASM^pc := 10;
+      goto label$returnFalse;
+    }
+    call $MASM^step();
+
+  op'1$MASM~unboxObject:
+    op := ops[1];
+    call regs := $MASM~unboxObject(
+      valueRegs,
+      regs,
+      $valueReg#$MASM^Op~unboxObject(op),
+      $objectReg#$MASM^Op~unboxObject(op)
+    );
+
+  op'2$MASM~loadObjectProto:
+    op := ops[2];
+    call valueRegs := $MASM~loadObjectProto(
+      valueRegs,
+      regs,
+      $objectReg#$MASM^Op~loadObjectProto(op),
+      $protoReg#$MASM^Op~loadObjectProto(op)
+    );
+
+  label$loop:
+  op'3$MASM^branchTestNull:
+    op := ops[3];
+    call $MASM~branchTestNull'tmp'0 := $ValueReg~getValue(valueRegs, $valueReg#$MASM^Op~branchTestNull(op));
+    $MASM~branchTestNull'$value := $MASM~branchTestNull'tmp'0;
+    call $MASM~branchTestNull'tmp'1 := $Value~isNull($MASM~branchTestNull'$value);
+    if ($MASM~branchTestNull'tmp'1) {
+      //call $MASM^jump($label#$MASM^Op~branchTestNull(op));
+      //$MASM^pc := 10;
+      goto label$returnFalse;
+    }
+    call $MASM^step();
+
+  op'4$MASM~branchTestMagic:
+    op := ops[4];
+    call $MASM~branchTestMagic'tmp'0 := $ValueReg~getValue(valueRegs, $valueReg#$MASM^Op~branchTestMagic(op));
+    $MASM~branchTestMagic'$value := $MASM~branchTestMagic'tmp'0;
+    call $MASM~branchTestMagic'tmp'1 := $Value~isMagic($MASM~branchTestMagic'$value);
+    if ($MASM~branchTestMagic'tmp'1) {
+      //call $MASM^jump($label#$MASM^Op~branchTestMagic(op));
+      //$MASM^pc := 14;
+      goto label$failure;
+    }
+    call $MASM^step();
+
+  op'5$MASM~branchTestNotObject:
+    op := ops[5];
+    call $MASM~branchTestNotObject'tmp'0 := $ValueReg~getValue(valueRegs, $valueReg#$MASM^Op~branchTestNotObject(op));
+    $MASM~branchTestNotObject'$value := $MASM~branchTestNotObject'tmp'0;
+    call $MASM~branchTestNotObject'tmp'1 := $Value~isObject($MASM~branchTestNotObject'$value);
+    if (!$MASM~branchTestNotObject'tmp'1) {
+      //call $MASM^jump($label#$MASM^Op~branchTestNotObject(op));
+      //$MASM^pc := 10;
+      goto label$returnFalse;
+    }
+    call $MASM^step();
+
+  op'6$MASM~unboxObject:
+    op := ops[6];
+    assert is#$MASM^Op~unboxObject(op);
+    call regs := $MASM~unboxObject(
+      valueRegs,
+      regs,
+      $valueReg#$MASM^Op~unboxObject(op),
+      $objectReg#$MASM^Op~unboxObject(op)
+    );
+
+  op'7$MASM~branchTestObjectEq:
+    op := ops[7];
+    call $MASM~branchTestObjectEq'tmp'0 := $Reg~getObject(regs, $lhsReg#$MASM^Op~branchTestObjectEq(op));
+    $MASM~branchTestObjectEq'$lhs := $MASM~branchTestObjectEq'tmp'0;
+    call $MASM~branchTestObjectEq'tmp'1 := $Reg~getObject(regs, $rhsReg#$MASM^Op~branchTestObjectEq(op));
+    $MASM~branchTestObjectEq'$rhs := $MASM~branchTestObjectEq'tmp'1;
+    if ($MASM~branchTestObjectEq'$lhs == $MASM~branchTestObjectEq'$rhs) {
+      //call $MASM^jump($label#$MASM^Op~branchTestObjectEq(op));
+      //$MASM^pc := 12;
+      goto label$returnTrue;
+    }
+    call $MASM^step();
+
+  op'8$MASM~loadObjectProto:
+    op := ops[8];
+    call valueRegs := $MASM~loadObjectProto(
+      valueRegs,
+      regs,
+      $objectReg#$MASM^Op~loadObjectProto(op),
+      $protoReg#$MASM^Op~loadObjectProto(op)
+    );
+
+  op'9$MASM~jump:
+    op := ops[9];
+    //call $MASM^jump($label#$MASM^Op~jump(op));
+    //$MASM^pc := 3;
+    goto label$loop;
+
+  label$returnFalse:
+  op'10$MASM~storeBoolean:
+    op := ops[10];
+    call regs := $MASM~storeBoolean(
+      regs,
+      $boolean#$MASM^Op~storeBoolean(op),
+      $dstReg#$MASM^Op~storeBoolean(op)
+    );
+
+  op'11$MASM~jump:
+    op := ops[11];
+    //call $MASM^jump($label#$MASM^Op~jump(op));
+    //$MASM^pc := 13;
+    goto label$done;
+
+  label$returnTrue:
+  op'12$MASM~storeBoolean:
+    op := ops[12];
+    call regs := $MASM~storeBoolean(
+      regs,
+      $boolean#$MASM^Op~storeBoolean(op),
+      $dstReg#$MASM^Op~storeBoolean(op)
+    );
+
+  label$done:
+
+  label$failure:
+}
